Makefile
@@ -156,9 +156,8 @@ BACKEND=\
   Bounds.v Stacklayout.v Stacking.v Stackingproof.v \
   Asm.v Asmgen.v Asmgenproof0.v Asmgenproof1.v Asmgenproof.v \
   Asmrel.v AsmLinking.v \
-
-# Unusedglob.v
-# Unusedglobproof.v
+  Unusedglob.v \
+  Unusedglobproof.v
 
 # C front-end modules (in cfrontend/)
 
